silveroak-opentitan/aes/Acorn/CipherRound.v
@@ -33,24 +33,29 @@ Section WithCava.
   Context {signal} {semantics : Cava signal}.
   Context {monad: Monad cava}.
 
-  Context (sub_bytes:     signal state -> cava (signal state))
-          (shift_rows:    signal state -> cava (signal state))
-          (mix_columns:   signal state -> cava (signal state))
+  Context (sub_bytes:     signal Bit -> signal state -> cava (signal state))
+          (shift_rows:    signal Bit -> signal state -> cava (signal state))
+          (mix_columns:   signal Bit -> signal state -> cava (signal state))
           (add_round_key: signal key -> signal state -> cava (signal state)).
 
-  Definition cipher_round (input: signal state) (key : signal key)
+  Definition cipher_round
+             (is_decrypt : signal Bit) (input: signal state) (key : signal key)
     : cava (signal state) :=
-    (sub_bytes >=> shift_rows >=> mix_columns >=> add_round_key key) input.
+    (sub_bytes is_decrypt   >=>
+     shift_rows is_decrypt  >=>
+     mix_columns is_decrypt >=>
+     add_round_key key) input.
 
   Definition cipher
+        (is_decrypt : signal Bit) (* called op_i in OpenTitan *)
         (first_key last_key : signal key)
         (middle_keys : list (signal key))
         (input : signal state)
         : cava (signal state) :=
-    (add_round_key first_key         >=>
-     foldLM cipher_round middle_keys >=>
-     sub_bytes                       >=>
-     shift_rows                      >=>
+    (add_round_key first_key                      >=>
+     foldLM (cipher_round is_decrypt) middle_keys >=>
+     sub_bytes is_decrypt                         >=>
+     shift_rows is_decrypt                        >=>
      add_round_key last_key) input.
 
 End WithCava.
